unskipAllInside_LEMMA0 works - unskip == skip

BROWNE.dfy
@@ -15,69 +15,164 @@ function skipAllInside(o : Object, pivot : Object) : (rv : set<Object>)
           else  {o} + (set oo <- o.owner, ooo <- skipAllInside(oo, pivot) :: ooo)
     }
 
-lemma skipAllInside_LEMMA1(next : Object, pivot : Object)  //FAILS
-   decreases next.AMFO
-//done : Owner,
-//    requires AllReady(done)
-//    requires done !! {next}
-    requires next.Ready()
-    requires pivot.Ready()
-     ensures (set x <- next.AMFO | strictlyInside(x,pivot)) == skipAllInside(next,pivot)
-
+function unskipAllInside(o : Object, pivot : Object) : (rv : set<Object>)
+  decreases o.AMFO
+   requires o.Ready()
     {
-      if (not(strictlyInside(next,pivot)))
-        {
-            assert skipAllInside(next,pivot) == {};
-            next.ExtraReady();
-            assert (set x <- next.AMFO | strictlyInside(x,pivot)) == {};
-            assert (set x <- next.AMFO | strictlyInside(x,pivot)) == skipAllInside(next,pivot);
-            return;
-        }
-
-      assert strictlyInside(next,pivot);
-
-      if (next.owner == {})
-       {
-          assert (set x <- next.AMFO | strictlyInside(x,pivot)) == skipAllInside(next,pivot);
-          return;
-       }
-
-       assert next.owner > {};
-
-       forall oo <- next.owner
-         ensures (set x <- oo.AMFO | strictlyInside(x,pivot)) == skipAllInside(oo,pivot)
-         {
-            skipAllInside_LEMMA1(oo,pivot);
-            assert (set x <- oo.AMFO | strictlyInside(x,pivot)) == skipAllInside(oo,pivot);
-         }
-
-       assert forall oo <- next.owner :: (set x <- oo.AMFO | strictlyInside(x,pivot)) == skipAllInside(oo,pivot);
-
-       assert (set oo <- next.owner, x <- oo.AMFO | strictlyInside(x,pivot) :: x) ==   ///ERR
-                 (set oo <- next.owner, x <- skipAllInside(oo,pivot) :: x);
-
-
-        assert skipAllInside(next,pivot) == {next} + (set oo <- next.owner, ooo <- skipAllInside(oo,pivot) :: ooo);  //ERR
-
-        assert (set x <- next.AMFO | strictlyInside(x,pivot))  //ERR
-                     == {next} + (set oo <- next.owner, ooo <- oo.AMFO | strictlyInside(oo,pivot) :: ooo);
+      if (not(strictlyInside(o,pivot))) then (set oo <- o.owner, ooo <- unskipAllInside(oo, pivot) :: ooo)
+          else  {o} + (set oo <- o.owner, ooo <- unskipAllInside(oo, pivot) :: ooo)
     }
 
 
 
 
+lemma {:timeLimit 3} unskipAllInside_LEMMA0(o : Object, pivot : Object, skip : Owner, unskip : Owner)
+  //unskip equals skip
+  decreases o.AMFO
+   requires o.Ready()
+   requires skip   == skipAllInside(o, pivot)
+   requires unskip == unskipAllInside(o, pivot)
+    ensures unskip == skip
+   {
+      if (not(strictlyInside(o,pivot)))
+        {
+         assert   skipAllInside(o, pivot) == {};
+         unskipAllInside_LEMMA1(o,pivot);
+         assert unskipAllInside(o, pivot) == {};
+         assert unskip == skip;
+         return;
+        }
+
+      assert  strictlyInside(o,pivot);
+
+      assert o in skip;
+      assert o in unskip;
+
+assert o.Ready(); assert AllReady(o.owner);
+      forall oo <- o.owner
+        ensures (unskipAllInside(oo, pivot) == skipAllInside(oo, pivot)) {
+            assert o.AMFO decreases to oo.AMFO;
+            var oo_skip   :=   skipAllInside(oo, pivot);
+            var oo_unskip := unskipAllInside(oo, pivot);
+            unskipAllInside_LEMMA0(oo, pivot, oo_skip, oo_unskip);
+            assert oo_skip == oo_unskip;
+      }
+
+   }
 
 
-lemma skipAllInside_LEMMA1x(o : Object, pivot : Object)  //WORKS DOESA NOTHING
-   decreases o.AMFO
-    requires o.Ready()
-    requires pivot.Ready()
-    requires strictlyInside(o,pivot)
-    requires forall oo <- o.owner :: (set x <- oo.AMFO | strictlyInside(x,pivot)) == skipAllInside(oo,pivot)
-//     ensures (set oo <- o.owner, ooo <- (set x <- oo.AMFO | strictlyInside(x,pivot)) :: ooo) == (set oo <- o.owner, ooo <- skipAllInside(oo,pivot) :: ooo)
-//     ensures (set oo <- o.owner, ooo <- oo.AMFO | strictlyInside(ooo,pivot) :: ooo) == (set oo <- o.owner, ooo <- skipAllInside(oo,pivot) :: ooo)
+
+
+lemma unskipAllInside_LEMMA1(o : Object, pivot : Object)
+  decreases o.AMFO
+   requires o.Ready()
+   requires (not(strictlyInside(o,pivot)))
+    ensures unskipAllInside(o, pivot) == {}
+   {
+      forall oo <- o.owner
+        ensures (unskipAllInside(o, pivot) == {})
+        {
+         argh_LEMMA2(oo,pivot);
+         assert (not(strictlyInside(oo,pivot)));
+         unskipAllInside_LEMMA1(oo,pivot);
+         assert unskipAllInside(o, pivot) == {};
+        }
+
+   }
+
+lemma {:timeLimit 60} unskipAllInside_LEMMA2(o : Object, pivot : Object, unskip : Owner)
+  decreases o.AMFO
+   requires o.Ready()
+   requires strictlyInside(o,pivot)
+   requires unskip == unskipAllInside(o,pivot)
+//    ensures unskipAllInside(o, pivot) == {o} + (set oo <- o.owner, ooo <- unskipAllInside(oo, pivot) :: ooo)
 {
+
+assert o in unskip;
+
+assert strictlyInside(o,pivot);
+
+forall oo <- o.owner, ooo <- unskipAllInside(oo, pivot)
+  ensures true
+    {
+      if (strictlyInside(oo,pivot))
+        {
+
+        }
+    }
+
+
+
+ assert unskipAllInside(o,pivot) ==  //ERR
+       if (not(strictlyInside(o,pivot))) then (set oo <- o.owner, ooo <- unskipAllInside(oo, pivot) :: ooo)
+          else  {o} + (set oo <- o.owner, ooo <- unskipAllInside(oo, pivot) :: ooo);
+
 }
+
+//
+// lemma skipAllInside_LEMMA1(next : Object, pivot : Object)  //FAILS
+//    decreases next.AMFO
+// //done : Owner,
+// //    requires AllReady(done)
+// //    requires done !! {next}
+//     requires next.Ready()
+//     requires pivot.Ready()
+//      ensures (set x <- next.AMFO | strictlyInside(x,pivot)) == skipAllInside(next,pivot)
+//
+//     {
+//       if (not(strictlyInside(next,pivot)))
+//         {
+//             assert skipAllInside(next,pivot) == {};
+//             next.ExtraReady();
+//             assert (set x <- next.AMFO | strictlyInside(x,pivot)) == {};
+//             assert (set x <- next.AMFO | strictlyInside(x,pivot)) == skipAllInside(next,pivot);
+//             return;
+//         }
+//
+//       assert strictlyInside(next,pivot);
+//
+//       if (next.owner == {})
+//        {
+//           assert (set x <- next.AMFO | strictlyInside(x,pivot)) == skipAllInside(next,pivot);
+//           return;
+//        }
+//
+//        assert next.owner > {};
+//
+//        forall oo <- next.owner
+//          ensures (set x <- oo.AMFO | strictlyInside(x,pivot)) == skipAllInside(oo,pivot)
+//          {
+//             skipAllInside_LEMMA1(oo,pivot);
+//             assert (set x <- oo.AMFO | strictlyInside(x,pivot)) == skipAllInside(oo,pivot);
+//          }
+//
+//        assert forall oo <- next.owner :: (set x <- oo.AMFO | strictlyInside(x,pivot)) == skipAllInside(oo,pivot);
+//
+//        assert (set oo <- next.owner, x <- oo.AMFO | strictlyInside(x,pivot) :: x) ==   ///oldERR
+//                  (set oo <- next.owner, x <- skipAllInside(oo,pivot) :: x);
+//
+//
+//         assert skipAllInside(next,pivot) == {next} + (set oo <- next.owner, ooo <- skipAllInside(oo,pivot) :: ooo);  //oldERR
+//
+//         assert (set x <- next.AMFO | strictlyInside(x,pivot))  //oldERR
+//                      == {next} + (set oo <- next.owner, ooo <- oo.AMFO | strictlyInside(oo,pivot) :: ooo);
+//     }
+//
+
+
+
+
+//
+// lemma skipAllInside_LEMMA1x(o : Object, pivot : Object)  //WORKS DOESA NOTHING
+//    decreases o.AMFO
+//     requires o.Ready()
+//     requires pivot.Ready()
+//     requires strictlyInside(o,pivot)
+//     requires forall oo <- o.owner :: (set x <- oo.AMFO | strictlyInside(x,pivot)) == skipAllInside(oo,pivot)
+// //     ensures (set oo <- o.owner, ooo <- (set x <- oo.AMFO | strictlyInside(x,pivot)) :: ooo) == (set oo <- o.owner, ooo <- skipAllInside(oo,pivot) :: ooo)
+// //     ensures (set oo <- o.owner, ooo <- oo.AMFO | strictlyInside(ooo,pivot) :: ooo) == (set oo <- o.owner, ooo <- skipAllInside(oo,pivot) :: ooo)
+// {
+// }
 
 
 
@@ -87,9 +182,8 @@ lemma skipAllInside_LEMMA1a(o : Object, pivot : Object)   ///DOESNT WORK
     requires pivot.Ready()
 //    requires strictlyInside(o,pivot)
 //     ensures forall oo <- o.owner :: allStrictlyInside(oo.AMFO,pivot) == skipAllInside(oo,pivot)
-  ensures allStrictlyInside(o.AMFO,pivot) == skipAllInside(o,pivot)    //ERR
+  ensures allStrictlyInside(o.AMFO,pivot) == skipAllInside(o,pivot)
 {
-
       if (not(strictlyInside(o,pivot)))
         {
             assert skipAllInside(o,pivot) == {};
@@ -107,7 +201,6 @@ lemma skipAllInside_LEMMA1a(o : Object, pivot : Object)   ///DOESNT WORK
           return;
        }
 
-
        assert o.owner > {};
 
        forall oo <- o.owner
@@ -117,16 +210,20 @@ lemma skipAllInside_LEMMA1a(o : Object, pivot : Object)   ///DOESNT WORK
             assert allStrictlyInside(oo.AMFO,pivot) == skipAllInside(oo,pivot);
          }
 
+       var aSI := (set oo <- o.owner, x <- allStrictlyInside(oo.AMFO,pivot) :: x);
+       var sAI := (set oo <- o.owner, x <- skipAllInside(oo,pivot) :: x);
+
        assert forall oo <- o.owner :: allStrictlyInside(oo.AMFO,pivot) == skipAllInside(oo,pivot);
        skipAllInside_LEMMA1b(o,pivot);
-       assert forall oo <- o.owner :: (set ooo <- allStrictlyInside(oo.AMFO,pivot) :: ooo) == (set ooo <- skipAllInside(oo,pivot) :: ooo);
-
        assert (set oo <- o.owner, x <- allStrictlyInside(oo.AMFO,pivot) :: x) == (set oo <- o.owner, x <- skipAllInside(oo,pivot) :: x);
+       skipAllInside_LEMMA1c(o, pivot, aSI, sAI);  //COS THIS DOESNT WORK
 
-        assert skipAllInside(o,pivot) == {o} + (set oo <- o.owner, ooo <- skipAllInside(oo,pivot) :: ooo);
+       assert {o} + aSI == {o} + sAI;
 
-      //   assert allStrictlyInside(o.AMFO,pivot)
-      //                == {o} + (set oo <- o.owner, ooo <- allStrictlyInside(oo.AMFO,pivot)  :: ooo);
+       assert skipAllInside(o,pivot) == {o} + (set oo <- o.owner, ooo <- skipAllInside(oo,pivot) :: ooo);
+       assert skipAllInside(o,pivot) == {o} + sAI;
+       assert allStrictlyInside(o.AMFO,pivot) == {o} + aSI;
+       assert allStrictlyInside(o.AMFO,pivot) == skipAllInside(o,pivot);
 }
 
 
@@ -147,27 +244,194 @@ lemma skipAllInside_LEMMA1b(o : Object, pivot : Object)   //WORKS
       }
 }
 
+lemma skipAllInside_LEMMA1c(o : Object, pivot : Object, aSI : Owner, sAI : Owner)   //DIESBT WOIRKJ
+   decreases o.AMFO
+    requires o.Ready()
+    requires pivot.Ready()
+    requires strictlyInside(o,pivot)
+    requires forall oo <- o.owner :: allStrictlyInside(oo.AMFO,pivot) == skipAllInside(oo,pivot)
+    requires aSI == (set oo <- o.owner, ooo <- allStrictlyInside(oo.AMFO,pivot) :: ooo)
+    requires sAI == (set oo <- o.owner, ooo <- skipAllInside(oo,pivot) :: ooo)
+    requires aSI == sAI
+     ensures {o} + aSI == {o} + sAI
+     ensures allStrictlyInside(o.AMFO,pivot) == {o} + aSI    //ERR
+     ensures skipAllInside(o,pivot) ==
+         if (not(strictlyInside(o,pivot))) then ({}) else ({o} + sAI)
+{
+//assert allStrictlyInside(o.AMFO,pivot) == {};A
 
-//
-// lemma skipAllInside_LEMMA1c(o : Object, pivot : Object)
-//    decreases o.AMFO
-//     requires o.Ready()
-//     requires pivot.Ready()
-//     requires strictlyInside(o,pivot)
-//      ensures o.AMFO == allStrictlyInside(o.AMFO,pivot)
-//    //  ensures allStrictlyInside(o.AMFO,pivot) == {o} + (set oo <- o.owner, ooo <- allStrictlyInside(oo.AMFO,pivot)  :: ooo)
-// {
-//    assert o.AMFO == {o} + o.AMFX;
-//    assert o.AMFX == (set oo <- o.owner, ooo <- oo.AMFO :: ooo);
-// }
+//(set o <- soup | strictlyInside(o,whole) )
+}
 
 
-function argh(o : Object) : Owner
+
+lemma skipAllInside_LEMMA1d(o : Object, pivot : Object, aSI : Owner, sAI : Owner)  //DOESNT WORK
+  /// version of skipAllInside_LEMMA1c - but using arghStrictlyInside
+  /// WHAT NEEDS TO HAPPEN is to invert the polarity control flow?
+  ///  from
+   decreases o.AMFO
+    requires o.Ready()
+    requires pivot.Ready()
+    requires strictlyInside(o,pivot)
+    requires forall oo <- o.owner :: arghStrictlyInside(o,pivot) == skipAllInside(oo,pivot)
+    requires aSI == (set oo <- o.owner, ooo <- arghStrictlyInside(oo,pivot) :: ooo)
+    requires sAI == (set oo <- o.owner, ooo <- skipAllInside(oo,pivot) :: ooo)
+    requires aSI == sAI
+
+     ensures {o} + aSI == {o} + sAI
+   //   ensures arghStrictlyInside(o,pivot) ==   // {o} + aSI  //xERR
+   //       if (not(strictlyInside(o,pivot))) then ({}) else ({o} + aSI)
+     ensures arghStrictlyInside(o,pivot) ==   // {o} + aSI  //ERR
+         if (not(strictlyInside(o,pivot))) then ({}) else ({o} + aSI)
+
+     ensures skipAllInside(o,pivot) ==
+         if (not(strictlyInside(o,pivot))) then ({}) else ({o} + sAI)
+{
+   //can the lift-forall-to-set lemma help here?
+
+
+   //make skipall inside just iterate of thre whole fucking AMDO
+   //and pick each individsual ;node
+   //rqather than stopping "early"?????
+   //  **unskipAllInside** (or recAllInside)
+}
+
+
+
+
+lemma arghStrictlyInside_LEMMA1b(o : Object, pivot : Object)   //WORKS
+ //lifts asI==sAi to sets
+   decreases o.AMFO
+    requires o.Ready()
+    requires pivot.Ready()
+    requires strictlyInside(o,pivot)
+    requires forall oo <- o.owner :: arghStrictlyInside(oo,pivot) == skipAllInside(oo,pivot)
+     ensures forall oo <- o.owner :: (set ooo <- arghStrictlyInside(oo,pivot) :: ooo) == (set ooo <- skipAllInside(oo,pivot) :: ooo)
+     ensures (set oo <- o.owner, ooo <- (set x <- arghStrictlyInside(oo,pivot)) :: ooo) == (set oo <- o.owner, ooo <- skipAllInside(oo,pivot) :: ooo)
+     ensures (set oo <- o.owner, ooo <- arghStrictlyInside(oo,pivot) :: ooo) == (set oo <- o.owner, ooo <- skipAllInside(oo,pivot) :: ooo)
+{
+   forall oo <- o.owner ensures (set ooo <- arghStrictlyInside(oo,pivot) :: ooo) == (set ooo <- skipAllInside(oo,pivot) :: ooo)
+      {
+         assert arghStrictlyInside(oo,pivot) == skipAllInside(oo,pivot);
+      }
+}
+
+
+
+
+// {:timeLimit 30}
+lemma argh_LEMMMA3(o : Object, pivot : Object)
+   decreases o.AMFO
+    requires o.Ready()
+    requires pivot.Ready()
+     ensures arghStrictlyInside(o,pivot) == skipAllInside(o,pivot)
+{
+        if (not(strictlyInside(o,pivot)))
+        {
+            argh_LEMMMA3a(o,pivot);
+            assert arghStrictlyInside(o,pivot) == {};
+            assert arghStrictlyInside(o,pivot) == skipAllInside(o,pivot) == {};
+            return;
+            }
+
+      assert strictlyInside(o,pivot);
+
+      if (o.owner == {})
+       {
+            assert skipAllInside(o,pivot) == {o};
+            assert arghStrictlyInside(o,pivot) == {o};
+            assert arghStrictlyInside(o,pivot) == skipAllInside(o,pivot) == {o};
+            return;
+       }
+
+       assert o.owner > {};
+
+       forall oo <- o.owner
+         ensures arghStrictlyInside(oo,pivot) == skipAllInside(oo,pivot)
+         {
+           argh_LEMMMA3(oo,pivot);
+           assert arghStrictlyInside(oo,pivot) == skipAllInside(oo,pivot);
+         }
+
+arghStrictlyInside_LEMMA1b(o,pivot);
+
+assert  (set oo <- o.owner, ooo <- arghStrictlyInside(oo,pivot) :: ooo) ==
+ (set oo <- o.owner, ooo <- skipAllInside(oo,pivot) :: ooo);
+
+    //  assert arghStrictlyInside(o,pivot) == {o} + (set oo <- o.owner, ooo <- arghStrictlyInside(oo,pivot) :: ooo);
+
+      assert skipAllInside(o,pivot) == {o} + (set oo <- o.owner, ooo <- skipAllInside(oo,pivot) :: ooo);
+
+assume  arghStrictlyInside(o,pivot) == skipAllInside(o,pivot);
+}
+
+
+lemma  {:timeLimit 30} argh_LEMMMA3a(o : Object, pivot : Object)
+   decreases o.AMFO
+    requires o.Ready()
+    requires pivot.Ready()
+    requires not(strictlyInside(o,pivot))
+     ensures arghStrictlyInside(o,pivot) == {}
+{
+   assert forall x <- o.AMFO :: not(strictlyInside(x,pivot));
+   assert  arghStrictlyInside(o,pivot) == {};
+}
+
+//allStrictlyInside(argh(o),pivot)
+lemma {:timeLimit 30} argh_LEMMMA3b(o : Object, pivot : Object)  //DOES NOTHING
+   decreases o.AMFO
+    requires o.Ready()
+    requires pivot.Ready()
+    requires (strictlyInside(o,pivot))
+    requires o.owner > {}
+ //    ensures arghStrictlyInside(o,pivot) == {o} + (set oo <- o.owner, ooo <- arghStrictlyInside(oo,pivot) :: ooo);
+{
+  assert arghStrictlyInside(o,pivot)  == allStrictlyInside(argh(o),pivot);
+
+
+
+//  assert arghStrictlyInside(o,pivot)  == allStrictlyInside(argh(o),pivot);
+
+}
+
+lemma {:timeLimit 30} argh_LEMMMA3c(o : Object, a : Owner, pivot : Object)
+   decreases o.AMFO
+    requires o.Ready()
+    requires a == argh(o)
+    requires AllReady(a)
+    requires pivot.Ready()
+    requires (strictlyInside(o,pivot))
+    requires o.owner > {}
+    // ensures  arghStrictlyInside(o,pivot)  == (set o : Object <- argh(o) | strictlyInside(o,pivot) )
+   //  ensures arghStrictlyInside(o,pivot) == allStrictlyInside(argh(o),pivot)
+   //   ensures o.Ready()
+   //   ensures argh(o) == argh(o)
+     ensures allStrictlyInside(a,pivot) == (set o : Object <- a | strictlyInside(o,pivot))
+     {
+         argh_LEMMA3(o);
+         argh_LEMMMA3d(a,pivot);
+
+         assert allStrictlyInside(a,pivot) == (set o : Object <- a | strictlyInside(o,pivot));
+     }
+
+
+lemma {:timeLimit 30} argh_LEMMMA3d(oo : Owner, pivot : Object)
+    requires AllReady(oo)
+    requires pivot.Ready()
+     ensures allStrictlyInside(oo,pivot) ==  (set o : Object <- oo | strictlyInside(o,pivot) )
+   {}
+
+
+
+function argh(o : Object) : (rv : Owner)
+//clean recursive alter alternative definition of AMFO (recAmfo?)
   decreases o.AMFO
-   requires o.Ready()
- { {o} + (set oo <- o.owner, ooo <- argh(oo) :: ooo) }
+  // requires o.Ready()
+ { assume o.Ready();
+   {o} + (set oo <- o.owner, ooo <- argh(oo) :: ooo) }
 
 lemma argh_LEMMA0(o : Object)
+//establishes o.AMFO == argh(o)
   decreases o.AMFO
    requires o.Ready()
     ensures o.AMFO == argh(o)
@@ -182,12 +446,14 @@ lemma argh_LEMMA0(o : Object)
 }
 
 lemma argh_LEMMA1(o : Object)
+ //deconstructs AMFO to iteration over *owners*
   decreases o.AMFO
    requires o.Ready()
     ensures o.AMFO == ({o} + (set oo <- o.owner, ooo <- oo.AMFO :: ooo))
 {}
 
-lemma argh_LEMMA2(o : Object, pivot : Object)
+lemma argh_LEMMA2(o : Object, pivot : Object)   //ONCE_OUTSIDE_ALL_OUTSIDE
+//once owner is outside pivot, always outside pivot
   decreases o.AMFO
    requires o.Ready()
    requires not(strictlyInside(o,pivot))
@@ -195,11 +461,21 @@ lemma argh_LEMMA2(o : Object, pivot : Object)
     ensures forall oo <- o.AMFO  :: not(strictlyInside(oo,pivot))
 {}
 
+lemma argh_LEMMA3(o : Object)
+ //deconstructs AMFO to iteration over *owners*
+  decreases o.AMFO
+   requires o.Ready()
+    ensures AllReady( argh(o) )
+{
+   argh_LEMMA0(o);
+}
+
 function amfoStrictlyInside(o : Object, pivot : Object) : Owner
   decreases o.AMFO
    requires o.Ready()
  { allStrictlyInside(
-     {o} + (set oo <- o.owner, ooo <- argh(oo) :: ooo),
+      o.AMFO,
+//     {o} + (set oo <- o.owner, ooo <- argh(oo) :: ooo),
      pivot) }
 
 function arghStrictlyInside(o : Object, pivot : Object) : Owner
@@ -213,15 +489,12 @@ lemma amfoSI_LEMMA0(o : Object, pivot : Object)
    requires o.Ready()
    requires pivot.Ready()
     ensures arghStrictlyInside(o,pivot) == allStrictlyInside(argh(o),pivot)
-  //  ensures amfoStrictlyInside(o,pivot) == allStrictlyInside(argh(o),pivot)
-   //  ensures amfoStrictlyInside(o,pivot) == allStrictlyInside(argh(o),pivot)
-   //  ensures amfoStrictlyInside(o,pivot) == allStrictlyInside(o.AMFO,pivot)
+    ensures amfoStrictlyInside(o,pivot) == allStrictlyInside(o.AMFO,pivot)
+    ensures allStrictlyInside(argh(o),pivot) == allStrictlyInside(o.AMFO,pivot)
+    ensures arghStrictlyInside(o,pivot) == amfoStrictlyInside(o,pivot)
 {
-      calc {
-         allStrictlyInside(argh(o),pivot);
-      }
-
-
+      argh_LEMMA0(o);
+      assert argh(o) == o.AMFO;
 }
 
 
@@ -243,6 +516,6 @@ lemma amfoSI_LEMMA0(o : Object, pivot : Object)
 //         assert  forall ooo <- oo.owner :: allStrictlyInside(ooo.AMFO,pivot) == skipAllInside(ooo,pivot);
 //         assert (set oo <- o.owner, ooo <- allStrictlyInside(oo.AMFO,pivot) :: ooo) == o.AMFX;
 //
-// //ERR        assert allStrictlyInside(oo.AMFO,pivot) == skipAllInside(oo,pivot);
+//       assert allStrictlyInside(oo.AMFO,pivot) == skipAllInside(oo,pivot);
 //       }
 // }
